coq/thieleuniversal/coqproofs/ZCPULemmas.v
@@ -1,0 +1,219 @@
+Require Import List.
+Require Import Lia.
+Require Import ThieleUniversal.
+
+Import ListNotations.
+Import CPU.
+
+(* Basic properties of register and memory operations. *)
+
+Lemma read_reg_write_same :
+  forall r v st,
+    r <= length (regs st) ->
+    read_reg r (write_reg r v st) = v.
+Proof.
+  intros r v st Hlen.
+  unfold read_reg, write_reg.
+  generalize (regs st) as l.
+  intros l.
+  revert r Hlen.
+  induction l as [|x l IH]; intros [|r] Hlen; simpl in *; try lia; auto.
+  - apply IH. lia.
+Qed.
+
+Lemma read_reg_write_other :
+  forall r1 r2 v st,
+    r1 <> r2 ->
+    read_reg r2 (write_reg r1 v st) = read_reg r2 st.
+Proof.
+  intros r1 r2 v st Hneq.
+  unfold read_reg, write_reg.
+  generalize (regs st) as l.
+  intros l.
+  revert r1 r2 Hneq.
+  induction l as [|x l IH]; intros [|r1] [|r2] Hneq; simpl; auto;
+    try (apply IH; congruence).
+Qed.
+
+Lemma read_mem_write_mem_same :
+  forall addr v st,
+    read_mem addr (write_mem addr v st) = v.
+Proof.
+  intros addr v st.
+  unfold read_mem, write_mem.
+  generalize (mem st) as m.
+  intros m.
+  revert addr.
+  induction m as [|x m IH]; intros [|addr]; simpl; auto.
+Qed.
+
+Lemma read_mem_write_mem_other :
+  forall a1 a2 v st,
+    a1 <> a2 ->
+    read_mem a2 (write_mem a1 v st) = read_mem a2 st.
+Proof.
+  intros a1 a2 v st Hneq.
+  unfold read_mem, write_mem.
+  generalize (mem st) as m.
+  intros m.
+  revert a1 a2 Hneq.
+  induction m as [|x m IH]; intros [|a1] [|a2] Hneq; simpl; auto;
+    try (apply IH; congruence).
+Qed.
+
+Lemma read_mem_write_reg :
+  forall addr r v st,
+    read_mem addr (write_reg r v st) = read_mem addr st.
+Proof.
+  intros addr r v st. unfold read_mem, write_reg. reflexivity.
+Qed.
+
+Lemma run1_preserves_memory :
+  forall st addr,
+    let pc := read_reg REG_PC st in
+    let instr := decode_instr (read_mem pc st) in
+    is_not_StoreIndirect instr ->
+    read_mem addr (run1 st) = read_mem addr st.
+Proof.
+  intros st addr pc instr Hns.
+  unfold run1.
+  unfold CPU.step.
+  remember (read_reg REG_PC st) as pc0.
+  remember (write_reg REG_PC (S pc0) st) as st'.
+  destruct instr; simpl in Hns; try contradiction;
+    try (rewrite read_mem_write_reg; reflexivity);
+    try (rewrite read_mem_write_reg; rewrite read_mem_write_reg; reflexivity).
+  - (* Jz case *)
+    destruct (Nat.eqb (read_reg rc st) 0);
+      rewrite read_mem_write_reg; reflexivity.
+  - (* Jnz case *)
+    destruct (Nat.eqb (read_reg rc st) 0);
+      repeat rewrite read_mem_write_reg; reflexivity.
+  - (* Halt case *)
+    reflexivity.
+Qed.
+
+(* Instructions that do not write to memory. *)
+Definition is_not_StoreIndirect (i:Instr) : Prop :=
+  match i with
+  | StoreIndirect _ _ => False
+  | _ => True
+  end.
+
+(* Running instructions that never store preserves memory outside the program area. *)
+Lemma run_n_preserves_memory_outside_range :
+  forall st n start_addr end_addr,
+    (forall i, i < n ->
+       let current_pc := read_reg REG_PC (run_n st i) in
+       let instr := decode_instr (read_mem current_pc st) in
+       is_not_StoreIndirect instr) ->
+    (forall addr, start_addr <= addr -> addr < end_addr ->
+       read_mem addr (run_n st n) = read_mem addr st).
+Proof.
+  induction n as [|n IH]; intros start_addr end_addr Hsafe addr Hge Hlt; simpl.
+  - reflexivity.
+  - assert (Hns :
+        let pc := read_reg REG_PC st in
+        let instr := decode_instr (read_mem pc st) in
+        is_not_StoreIndirect instr).
+    { specialize (Hsafe 0). apply Hsafe. lia. }
+    assert (Hmem1 : forall a, read_mem a (run1 st) = read_mem a st).
+    { intro a. apply run1_preserves_memory with (st:=st) (addr:=a).
+      unfold is_not_StoreIndirect in Hns. exact Hns. }
+    assert (Hsafe' : forall i, i < n ->
+        let current_pc := read_reg REG_PC (run_n (run1 st) i) in
+        let instr := decode_instr (read_mem current_pc (run1 st)) in
+        is_not_StoreIndirect instr).
+    { intros i Hi.
+      specialize (Hsafe (S i)). assert (S i < S n) by lia. specialize (Hsafe H0).
+      rewrite run_n_succ in Hsafe.
+      set (pc := read_reg REG_PC (run_n (run1 st) i)) in *.
+      rewrite <- (Hmem1 pc) in Hsafe. exact Hsafe. }
+    rewrite run_n_succ.
+    specialize (IH start_addr end_addr Hsafe' addr Hge Hlt).
+    rewrite IH.
+    apply Hmem1.
+Qed.
+
+(* Encoding rules occupy five consecutive cells per TM rule. *)
+Lemma length_encode_rule : forall r,
+  length (encode_rule r) = 5.
+Proof.
+  intros [q [s [q' [w m]]]]. simpl. reflexivity.
+Qed.
+
+Lemma length_encode_rules : forall rs,
+  length (encode_rules rs) = 5 * length rs.
+Proof.
+  induction rs as [|r rs IH]; simpl; auto.
+  rewrite app_length, length_encode_rule, IH. lia.
+Qed.
+
+Lemma nth_encode_rules :
+  forall rs i j d,
+    i < length rs -> j < 5 ->
+    nth (i * 5 + j) (encode_rules rs) d =
+    match nth i rs (0,0,0,0,0%Z) with
+    | (q_rule, sym_rule, q_next, w_next, m_next) =>
+        match j with
+        | 0 => q_rule
+        | 1 => sym_rule
+        | 2 => q_next
+        | 3 => w_next
+        | _ => encode_z m_next
+        end
+    end.
+Proof.
+  induction rs as [|r rs IH]; intros i j d Hi Hj; simpl in *; try lia.
+  destruct i.
+  - destruct r as [q_rule [sym_rule [q_next [w_next m_next]]]].
+    destruct j; simpl in *; try lia; try reflexivity.
+    destruct j; simpl in *; try lia; try reflexivity.
+    destruct j; simpl in *; try lia; try reflexivity.
+    destruct j; simpl in *; try lia; try reflexivity.
+    destruct j; simpl in *; try lia; try reflexivity.
+  - replace (S i * 5 + j) with (5 + (i * 5 + j)) by lia.
+    rewrite flat_map_cons, nth_app.
+    rewrite length_encode_rule.
+    destruct (lt_dec (i * 5 + j) (length (encode_rules rs))).
+    + rewrite IH; try lia.
+      destruct (nth i rs (0,0,0,0,0%Z)) as [[[[q1 s1] q1'] w1'] m1'].
+      simpl. destruct j; simpl in *; try lia; reflexivity.
+    + assert (i * 5 + j < 5 + length (encode_rules rs)) by (rewrite length_encode_rule; lia).
+      exfalso. apply n. lia.
+Qed.
+
+(* Bridge between abstract rule list and concrete memory layout. *)
+Lemma read_mem_rule_component :
+  forall tm conf st i component_offset,
+    inv st tm conf ->
+    i < length (tm_rules tm) ->
+    let rule_addr := RULES_START_ADDR + i * 5 + component_offset in
+    let rule_list := tm_rules tm in
+    let '(q_rule, sym_rule, q_next, w_next, m_next) :=
+        nth i rule_list (0,0,0,0,0%Z) in
+    (component_offset = 0 -> read_mem rule_addr st = q_rule) /\
+    (component_offset = 1 -> read_mem rule_addr st = sym_rule) /\
+    (component_offset = 2 -> read_mem rule_addr st = q_next) /\
+    (component_offset = 3 -> read_mem rule_addr st = w_next) /\
+    (component_offset = 4 -> read_mem rule_addr st = encode_z m_next).
+Proof.
+  intros tm conf st i component_offset Hinv Hi.
+  unfold rule_addr, rule_list.
+  destruct Hinv as [HQ [HHEAD [HPC [Htape [Hprog Hr]]]]].
+  set (rules := tm_rules tm) in *.
+  assert (Hr_mem : forall k,
+            k < length (encode_rules rules) ->
+            read_mem (RULES_START_ADDR + k) st = nth k (encode_rules rules) 0).
+  {
+    intros k Hk.
+    pose proof (f_equal (fun l => nth k l 0) Hr) as Hnth.
+    rewrite nth_firstn in Hnth by lia.
+    rewrite nth_skipn in Hnth.
+    exact Hnth.
+  }
+  repeat split; intros Hc; subst component_offset;
+    rewrite Hr_mem; try (rewrite length_encode_rules; lia);
+    rewrite nth_encode_rules with (rs:=rules) (i:=i);
+    try lia; reflexivity.
+Qed.
